src/dafny/utils/NonNativeTypes.dfy
@@ -30,5 +30,49 @@
     * positive numbers that can be expressed in binary form with no more than 256
     * bits 
     */
-    newtype uint256 = i:int | 0 <= i < power2(256)       
+    newtype uint256 = i:int | 0 <= i < power2(256)     
+
+
+    // The foollowing functions and lemmas are used by the Eth2Types module and
+    // are probably only requried because we currently define uint128 and
+    // uint256 uisng power2
+    function method castUin64ToUint256(x:uint64): uint256
+    ensures castUin64ToUint256(x) as nat < 0x10000000000000000
+    ensures castUin64ToUint256(x) as uint64 == x
+    {
+        UpperBoundForUint64(x);
+        lemmaPower2IsMonotnoic(64,256);
+        x as uint256
+    }
+
+    lemma UpperBoundForUint64(x:uint64)
+    ensures x as nat < power2(64)
+    {
+        calc ==>
+        {
+            0x100000000 == power2(32); 
+            0x10000000000000000 == power2(64);  
+        }
+    }
+
+    function method castUin128ToUint256(x:uint128): uint256
+    ensures castUin128ToUint256(x) as nat < power2(128)
+    ensures castUin128ToUint256(x) as uint128 == x    
+    {
+        UpperBoundForUint128(x);
+        lemmaPower2IsMonotnoic(128,256);
+        x as uint256
+    }   
+
+    lemma UpperBoundForUint128(x:uint128)
+    ensures x as nat < power2(128)
+    {
+        calc ==>
+        {
+            0x100000000 == power2(32); 
+            0x10000000000000000 == power2(64);  
+                { productRulePower2(64,64); }
+            0x100000000000000000000000000000000 == power2(128);
+        }
+    }     
  }
